theories/Prelude/Prelude.v
@@ -1032,18 +1032,18 @@ Inductive transitiveClosure {A : Type} (R : A -> A -> Prop) (x : A) (y : A) : Pr
     : transitiveClosure R x y
   | transitiveClosure_trans z
     (STEPs : transitiveClosure R x z)
-    (STEP : transitiveClosure R z y)
+    (STEPs' : transitiveClosure R z y)
     : transitiveClosure R x y.
 
 #[local] Hint Constructors transitiveClosure : core.
 
-Lemma transitiveClosure_lift_well_founded {A : Type} (R : A -> A -> Prop)
+Lemma transitiveClosure_lifts_well_founded {A : Type} (R : A -> A -> Prop)
   (R_wf : well_founded R)
   : well_founded (transitiveClosure R).
 Proof.
   intros x. pose proof (R_wf x) as H_ACC. clear R_wf.
   induction H_ACC as [x H_ACC_inv IH]. constructor 1.
-  induction 1 as [x y | x y z H1 IH1 H2 IH2]; eauto.
+  induction 1 as [x y R_x_y | x y z H1 IH1 H2 IH2]; eauto.
   eapply IH2; eauto.
 Qed.
 
