theories/Prelude/Quotient.v
@@ -1,18 +1,6 @@
 Require Export PnV.Prelude.Prelude.
-Require Export Stdlib.Logic.ChoiceFacts.
-Require Export Stdlib.Logic.ClassicalChoice.
+Require Export PnV.Prelude.ClassicalFacts.
 Require Export Stdlib.Logic.EqdepFacts.
-
-Module AxiomOfChoice.
-
-Lemma AC {A : Type} {B : A -> Type} (R : forall x : A, forall y : B x, Prop)
-  (EXISTENCE : forall x, exists y, R x y)
-  : exists f : forall x : A, B x, forall x, R x (f x).
-Proof.
-  eapply non_dep_dep_functional_choice; [exact choice | exact EXISTENCE].
-Defined.
-
-End AxiomOfChoice.
 
 Module Quot.
 
